##### $\forall n \in N^{*}, p \leq n,  \binom{n}{p} = \frac{n!}{p!(n-p)}$

$total = \binom{4}{3} \cdot \binom{7}{2} + \binom{4}{4} \cdot \binom{6}{1} - \binom{3}{2} \cdot \binom{6}{1} = 4 \times 21 + 1 \times 6 - 3 \times 6 =$
$\text{Exercice 1:}$
$f(x) = 2^{(x-1)^{2}+2}= e^{((x-1)^2+2)\ln(2)}$
$f'(x) = (2\ln(2)(x-1)^2)e^{((x-1)^2+2)\ln(2)}$
$f'(x) = 0 \iff 2\ln(2)(x-1)^{2}= 0 \iff (x-1)^{2} = 0 \iff x = 1$
$\text{Un Minimum de} f(x) \text{est donc atteint en } x = 1 \text{et sa valeur est } f(1) = 2^{2}= 4$.

$\text{Exercice 6:}$
$x^{2}42^{2} = 172(42x - 43) \iff 1764x^{2} - 7224x + 7396 = 0$

$\text{Exercice 3:}$
$z =\frac{1}{2+3i} = \frac{2-3i}{13}$
$\Im(z) + \Re(z) = \frac{-1}{13}$

$\text{Exercice 5:}$
$z = x + iy$
$\mid z \mid + \mid \bar{z} \mid = \mid z + \bar{z} \mid$
$\iff \sqrt{x^{2}+ y^{2}}+ \sqrt{x^{2}+(-y)^{2}} = \sqrt{(2x)^2}$
$\iff 2\sqrt{x^{2}+y^{2}}= 2\sqrt{x^2}$
$\iff y = 0 \iff \Im(z) = 0$


