$$
\begin{gathered}



z = 4 - 3i \\\\
c = x+iy\\
c^{2} = z \\\\
\iff


\begin{cases} 
x^{2}-y^{2}=4\\
2xy = 3\\
\end{cases}\\
\iff 
\begin{cases} 
x =\pm\sqrt{\frac{\sqrt{4^{2}+3^{2}}+4}{2}} \\
y = \pm\sqrt{\frac{\sqrt{4^{2}+3^{2}}-4}{2}}\\
\end{cases}\\
\end{gathered}
$$

$\triangle = 49 - 4\cdot3\cdot p$
$\triangle = 0 \iff p = \frac{49}{12}$

$P(x) = ax^{2}+ bx + c$
$P'(x) = 2ax + b$
$P'(k) = 0 \iff b = -2ak$

$(1 + i)^{20} = (\sqrt{2}e^{i\frac{\pi}{4}})^{20}$
$=1024e^{-i5\pi}$
$=1024\cos(\pi) + i1024\sin(\pi)$